symbolic system prototype for function call evaluation and experiment on bloomfilter

core/ConcreteHoare.v
@@ -9,6 +9,7 @@ Require Import Poulet4.V1Model.
 Require Import ProD3.core.V1ModelLang.
 Require Import Hammer.Tactics.Tactics.
 Require Import Hammer.Plugin.Hammer.
+Require Import Coq.ZArith.BinInt.
 
 Section ConcreteHoare.
 
@@ -40,7 +41,7 @@ Definition assertion : Type := mem_assertion * ext_assertion.
 
 Record post_assertion := mk_post_assertion {
   post_continue :> assertion;
-  post_return : ret_assertion * mem_assertion * ext_assertion
+  post_return : ret_assertion * (mem_assertion * ext_assertion)
 }.
 
 Definition to_shallow_assertion_continue (a : assertion) :=
@@ -50,8 +51,8 @@ Definition to_shallow_assertion_continue (a : assertion) :=
     ext_to_shallow_assertion this a_ext es)
   end.
 
-Definition to_shallow_assertion_return (a : ret_assertion * mem_assertion * ext_assertion) :=
-  match a with (a_ret, a_mem, a_ext) =>
+Definition to_shallow_assertion_return (a : ret_assertion * (mem_assertion * ext_assertion)) :=
+  match a with (a_ret, (a_mem, a_ext)) =>
   (fun vret (st : state) => let (m, es) := st in
     ret_to_shallow_assertion a_ret vret /\
     to_shallow_assertion this a_mem m /\
@@ -61,6 +62,28 @@ Definition to_shallow_assertion_return (a : ret_assertion * mem_assertion * ext_
 Definition to_shallow_post_assertion (post : post_assertion) : Hoare.post_assertion :=
   match post with mk_post_assertion a_continue a_return =>
   Hoare.mk_post_assertion (to_shallow_assertion_continue a_continue) (to_shallow_assertion_return a_return)
+  end.
+
+Definition to_shallow_arg_assertion (a : arg_assertion * (mem_assertion * ext_assertion)) : Hoare.arg_assertion :=
+  match a with (a_arg, (a_mem, a_ext)) =>
+  (fun args (st : state) =>
+    arg_to_shallow_assertion a_arg args /\
+    to_shallow_assertion_continue (a_mem, a_ext) st)
+  end.
+
+Definition to_shallow_arg_ret_assertion (a : arg_assertion * ret_assertion * (mem_assertion * ext_assertion)) : Hoare.arg_ret_assertion :=
+  match a with (a_arg, a_ret, (a_mem, a_ext)) =>
+  (fun args vret (st : state) =>
+    arg_to_shallow_assertion a_arg args /\
+    ret_to_shallow_assertion a_ret vret /\
+    to_shallow_assertion_continue (a_mem, a_ext) st)
+  end.
+
+Definition to_shallow_ret_assertion (a : ret_assertion * (mem_assertion * ext_assertion)) : Hoare.ret_assertion :=
+  match a with (a_ret, (a_mem, a_ext)) =>
+  (fun vret (st : state) =>
+    ret_to_shallow_assertion a_ret vret /\
+    to_shallow_assertion_continue (a_mem, a_ext) st)
   end.
 
 Definition implies (pre : assertion) (post : assertion) : bool :=
@@ -76,6 +99,12 @@ Proof.
   - eapply AssertionLangSoundness.implies_sound; eassumption.
   - eapply ext_implies_sound; eassumption.
 Qed.
+
+Lemma implies_refl : forall (a : assertion),
+  implies a a.
+Proof.
+  clear ge inst_m this. admit.
+Admitted.
 
 Definition hoare_expr (pre : assertion) (expr : Expression) (v : Val) : Prop :=
   eval_expr ge (fst pre) expr = Some v.
@@ -102,7 +131,7 @@ Proof.
 Qed.
 
 Definition hoare_write (pre : assertion) (lv : Lval) (v : Val) (post : assertion) : Prop :=
-  is_writable_lval lv (fst pre) /\ eval_write (fst pre) lv v = (fst post) /\ (snd pre = snd post).
+  is_writable_lval lv (fst pre) /\ (eval_write (fst pre) lv v, snd pre) = post.
 
 Lemma exec_write_preserve_extern_state : forall st lv v st',
   exec_write (H := V1Model) this st lv v st' ->
@@ -147,13 +176,175 @@ Inductive hoare_block : path -> assertion -> (@Block tags_t) -> post_assertion -
       hoare_block p mid rest post ->
       hoare_block p pre (BlockCons stmt rest) post.
 
+Definition option_to_list {A} (ox : option A) : list A :=
+  match ox with
+  | Some x => [x]
+  | None => nil
+  end.
+
+Definition eval_copy_in (pre : arg_assertion * assertion) (params : list Locator) : assertion :=
+  match pre with (pre_arg, (pre_mem, pre_ext)) =>
+    let pre_mem_1 := fold_left clear_loc params pre_mem in
+    let post_mem := fold_left
+        (fun post_mem a_unit => post_mem ++ option_to_list (arg_assertion_unit_to_assertion_unit params a_unit))
+        pre_arg
+        pre_mem_1 in
+    (post_mem, pre_ext)
+  end.
+
+Inductive hoare_copy_in : arg_assertion * assertion -> list Locator -> assertion -> Prop :=
+  | hoare_copy_in_intro : forall pre params post,
+      eval_copy_in pre params = post ->
+      hoare_copy_in pre params post.
+
+Fixpoint eval_outargs (* (pre : assertion) *) (dirs : list direction) (args : list (option Expression))
+    : option (list (option Lval)) :=
+  match dirs, args with
+  | [], [] => Some nil
+  | dir :: dirs, arg :: args =>
+      let olvs := eval_outargs (* pre *) dirs args in
+      match dir with
+      | Out | InOut =>
+          match arg with
+          | Some expr =>
+              match eval_lexpr expr with
+              | Some lv => option_map (cons (Some lv)) olvs
+              | None => None
+              end
+          | None => option_map (cons None) olvs
+          end
+      | _ => olvs
+      end
+  | _, _ => None
+  end.
+
+Inductive hoare_outargs : assertion -> list direction -> list (option Expression) -> list (option Lval) -> Prop :=
+  | hoare_outargs_intro : forall pre dirs args lvs,
+      eval_outargs dirs args = Some lvs ->
+      hoare_outargs pre dirs args lvs.
+
+(*   | exec_expr_name: forall name loc v this st tag typ dir,
+                    loc_to_val this loc st = Some v ->
+                    exec_expr this st
+                    (MkExpression tag (ExpName name loc) typ dir)
+                    v *)
+
+Definition assertion_unit_to_arg_assertion_unit (a_unit : @assertion_unit tags_t) (cnt : Z) : arg_assertion_unit :=
+  match a_unit with
+  | AVal (_, fl) v => ArgVal (cnt, fl) v
+  | AType (_, fl) typ => ArgType (cnt, fl) typ
+  end.
+
+Fixpoint filter_locator_replace (a : mem_assertion) (loc : Locator) (cnt : Z) : arg_assertion :=
+  match a with
+  | a_unit :: a =>
+      let loc' :=
+        match a_unit with
+        | AVal (loc', _) _ => loc'
+        | AType (loc', _) _ => loc'
+        end in
+      if locator_equivb loc' loc then
+        assertion_unit_to_arg_assertion_unit a_unit cnt :: filter_locator_replace a loc cnt
+      else
+        filter_locator_replace a loc cnt
+  | [] => []
+  end.
+
+Fixpoint eval_inargs (pre : assertion) (dirs : list direction) (args : list (option Expression)) (cnt : Z) : option arg_assertion :=
+  match dirs, args with
+  | [], [] => Some nil
+  | dir :: dirs, arg :: args =>
+      match dir with
+      | Typed.In | InOut =>
+          match arg with
+          | Some expr =>
+              match expr with
+              | MkExpression _ (ExpName _ loc) _ _ =>
+                  option_map (app (filter_locator_replace (fst pre) loc cnt)) (eval_inargs pre dirs args (cnt + 1))
+              | _ =>
+                  match eval_expr ge (fst pre) expr with
+                  | Some v => option_map (cons (ArgVal (cnt, []) v)) (eval_inargs pre dirs args (cnt + 1))
+                  | None => None
+                  end
+              end
+          | None => None
+          end
+      | _ => eval_inargs pre dirs args cnt
+      end
+  | _, _ => None
+  end.
+
+Inductive hoare_inargs : assertion -> list direction -> list (option Expression) -> arg_assertion * assertion -> Prop :=
+  | hoare_inargs_intro : forall pre dirs args post,
+      eval_inargs pre dirs args 0 = Some post ->
+      hoare_inargs pre dirs args (post, pre).
+
+Fixpoint eval_copy_out (pre : assertion) (params : list Locator) (cnt : Z) : arg_assertion :=
+  match params with
+  | param :: params =>
+      app (filter_locator_replace (fst pre) param cnt) (eval_copy_out pre params (cnt + 1))
+  | [] => []
+  end.
+
+Inductive hoare_copy_out : assertion -> list Locator -> arg_assertion * assertion -> Prop :=
+  | hoare_copy_out_intro : forall pre params post_arg,
+      eval_copy_out pre params 0 = post_arg ->
+      hoare_copy_out pre params (post_arg, pre).
+
+(* Definition eval_copy_in (pre : arg_assertion * assertion) (params : list Locator) : assertion :=
+  match pre with (pre_arg, (pre_mem, pre_ext)) =>
+    let pre_mem_1 := fold_left clear_loc params pre_mem in
+    let post_mem := fold_left
+        (fun post_mem a_unit => post_mem ++ option_to_list (arg_assertion_unit_to_assertion_unit params a_unit))
+        pre_arg
+        pre_mem_1 in
+    (post_mem, pre_ext)
+  end. *)
+
+(* Inductive hoare_copy_in : arg_assertion * assertion -> list Locator -> assertion -> Prop :=
+  | hoare_copy_in_intro : forall pre params post,
+      eval_copy_in pre params = post ->
+      hoare_copy_in pre params post. *)
+
+Fixpoint olvals_to_locs (outlvs : list (option Lval)) : option (list Locator) :=
+  match outlvs with
+  | lv :: outlvs =>
+      match lv with
+      | Some (loc, []) => option_map (cons loc) (olvals_to_locs outlvs)
+      | _ => None
+      end
+  | [] => Some []
+  end.
+
+Definition eval_write_copy_out (pre : arg_assertion * ret_assertion * assertion) (outlvs : list (option Lval)) : option (ret_assertion * assertion) :=
+  match olvals_to_locs outlvs with
+  | Some locs =>
+      match pre with (pre_arg, pre_ret, (pre_mem, pre_ext)) =>
+        let pre_mem_1 := fold_left clear_loc locs pre_mem in
+        let post_mem := fold_left
+            (fun post_mem a_unit => post_mem ++ option_to_list (arg_assertion_unit_to_assertion_unit locs a_unit))
+            pre_arg
+            pre_mem_1 in
+        Some (pre_ret, (post_mem, pre_ext))
+      end
+  | None => None
+  end.
+
+Inductive hoare_write_copy_out : arg_assertion * ret_assertion * assertion -> list (option Lval) -> ret_assertion * assertion -> Prop :=
+  | hoare_write_copy_out_intro : forall pre outlvs post,
+      eval_write_copy_out pre outlvs = Some post ->
+      hoare_write_copy_out pre outlvs post.
+
+Definition ret_assertion_to_assertion (a : ret_assertion * assertion) : assertion :=
+  snd a.
+
 Lemma hoare_stmt_sound : forall p pre stmt post,
   wellformed (fst pre) ->
   hoare_stmt p pre stmt post ->
   Hoare.deep_hoare_stmt ge inst_m p (to_shallow_assertion_continue p pre) stmt (to_shallow_post_assertion p post).
 Proof.
   intros * H_wellformed H_hoare_stmt.
-  apply deep_hoare_stmt_intro.
+  apply deep_hoare_stmt_fallback.
   induction H_hoare_stmt.
   - hnf. intros. pinv @exec_stmt.
     + assert (is_valid_field (fst pre) lv). {
@@ -189,5 +380,55 @@ Proof.
   - apply hoare_stmt_sound in H; only 2 : assumption.
     destruct mid; econstructor; eauto.
 Qed.
+
+Lemma hoare_copy_in_sound : forall p pre params post,
+  hoare_copy_in pre params post ->
+  Hoare.deep_hoare_copy_in p (to_shallow_arg_assertion p pre) params (to_shallow_assertion_continue p post).
+Proof.
+  clear ge inst_m.
+  admit.
+Admitted.
+
+Lemma hoare_outargs_sound : forall p pre dirs args lvs,
+  hoare_outargs pre dirs args lvs ->
+  Hoare.deep_hoare_outargs (H := V1Model) ge p (to_shallow_assertion_continue p pre) dirs args
+      (map (option_map lval_to_semlval) lvs).
+Proof.
+  clear inst_m.
+  admit.
+Admitted.
+
+Lemma hoare_inargs_sound : forall p pre dirs args post,
+  hoare_inargs pre dirs args post ->
+  Hoare.deep_hoare_inargs (H := V1Model) ge p (to_shallow_assertion_continue p pre) dirs args
+      (to_shallow_arg_assertion p post).
+Proof.
+  clear inst_m.
+  admit.
+Admitted.
+
+Lemma hoare_copy_out_sound : forall p pre params post,
+  hoare_copy_out pre params post ->
+  Hoare.implies (to_shallow_assertion_continue p pre) (return_post_assertion_1 (generate_post_condition p params (to_shallow_arg_ret_assertion p (fst post, [], snd post)))).
+Proof.
+  clear ge inst_m.
+  admit.
+Admitted.
+
+Lemma hoare_write_copy_out_sound : forall p pre outlvs post,
+  hoare_write_copy_out pre outlvs post ->
+  deep_hoare_write_copy_out p (to_shallow_arg_ret_assertion p pre) (map (option_map lval_to_semlval) outlvs) (to_shallow_ret_assertion p post) .
+Proof.
+  clear ge inst_m.
+  admit.
+Admitted.
+
+Lemma ret_assertion_to_assertion_sound : forall p pre post,
+  ret_assertion_to_assertion pre = post ->
+  Hoare.ret_assertion_to_assertion (to_shallow_ret_assertion p pre) = (to_shallow_assertion_continue p post).
+Proof.
+  clear ge inst_m.
+  admit.
+Admitted.
 
 End ConcreteHoare.
