examples/bloomfilter/verif.v
@@ -1,5 +1,6 @@
 Require Import Poulet4.P4defs.
 Require Import Poulet4.P4Notations.
+Require Import Coq.Program.Basics.
 Open Scope string_scope.
 
 Import ListNotations.
@@ -15,8 +16,6 @@ Require Import ProD3.core.HoareSoundness.
 Require Import ProD3.core.AssertionLang.
 Require Import ProD3.core.V1ModelLang.
 Require Import ProD3.core.ConcreteHoare.
-
-Require Import mathcomp.ssreflect.fintype.
 
 Instance target : @Target Info (@Expression Info) := V1Model.
 
@@ -54,33 +53,26 @@ Definition MyIngress_fundef := Eval compute in
 
 Definition this : path := !["main"; "ig"].
 
-Definition NUM_ENTRY : nat := 1024.
+Definition NUM_ENTRY : Z := 1024.
 
-Notation Filter := (Filter 'I_NUM_ENTRY).
+Notation Filter := (Filter Z).
 
 Definition bloomfilter_state : Type := Filter * Filter * Filter.
 
 Definition bool_to_Z (b : bool) :=
   if b then 1 else 0.
 
-Program Fixpoint list_of_filter (size : 'I_(S NUM_ENTRY)) (f : Filter) {measure (nat_of_ord size)} : list Z :=
-  match size with
-  | Ordinal O _ => nil
-  | Ordinal (S size') _ =>
-      list_of_filter (@Ordinal (S NUM_ENTRY) size' _) f ++
-          [bool_to_Z (f (@Ordinal _ size' _))]
-  end.
-
-Program Definition NUM_ENTRY_1 : 'I_(S NUM_ENTRY) := @Ordinal _ NUM_ENTRY _.
+Definition list_of_filter (size : Z) (f : Filter) : list Z :=
+  map (compose bool_to_Z (compose f Z.of_nat)) (seq O (Z.to_nat size)).
 
 Definition bloom0 (bst : bloomfilter_state) : list Z :=
-  list_of_filter NUM_ENTRY_1 (fst (fst bst)).
+  list_of_filter NUM_ENTRY (fst (fst bst)).
 
 Definition bloom1 (bst : bloomfilter_state) : list Z :=
-  list_of_filter NUM_ENTRY_1 (snd (fst bst)).
+  list_of_filter NUM_ENTRY (snd (fst bst)).
 
 Definition bloom2 (bst : bloomfilter_state) : list Z :=
-  list_of_filter NUM_ENTRY_1 (snd bst).
+  list_of_filter NUM_ENTRY (snd bst).
 
 (* Definition filter_match (st : state) (p : path) (f : Filter) : Prop :=
   exists content,
@@ -109,51 +101,148 @@ Variable bst : bloomfilter_state.
 Definition pre_arg_assertion : arg_assertion :=
   [
     ArgVal (0%Z, ["myHeader"; "rw"]) (ValBaseBit 8%nat rw);
-    ArgVal (0%Z, ["myHeader"; "data"]) (ValBaseBit 16%nat data)
+    ArgVal (0%Z, ["myHeader"; "data"]) (ValBaseBit 16%nat data);
+    ArgType (0%Z, []) (TypTypeName (BareName !"headers"));
+    ArgType (1%Z, []) (TypTypeName (BareName !"custom_metadata_t"));
+    ArgType (2%Z, []) (TypTypeName (BareName !"standard_metadata_t"))
   ].
 
 Definition pre_ext_assertion : ext_assertion :=
   [
-    (LGlobal !["bloom0"], ObjRegister (mk_register 1%nat (Z.of_nat NUM_ENTRY) (bloom0 bst)));
-    (LGlobal !["bloom1"], ObjRegister (mk_register 1%nat (Z.of_nat NUM_ENTRY) (bloom1 bst)));
-    (LGlobal !["bloom2"], ObjRegister (mk_register 1%nat (Z.of_nat NUM_ENTRY) (bloom2 bst)))
+    (LGlobal !["bloom0"], ObjRegister (mk_register 1%nat NUM_ENTRY (bloom0 bst)));
+    (LGlobal !["bloom1"], ObjRegister (mk_register 1%nat NUM_ENTRY (bloom1 bst)));
+    (LGlobal !["bloom2"], ObjRegister (mk_register 1%nat NUM_ENTRY (bloom2 bst)))
   ].
 
 Definition pre (args : list Val) (st : state) :=
   arg_to_shallow_assertion pre_arg_assertion args /\
-    ext_to_shallow_assertion this pre_ext_assertion (snd st).
+    to_shallow_assertion_continue this ([], pre_ext_assertion) st.
 
-Axiom CRC : Z -> 'I_NUM_ENTRY.
+Axiom CRC : Z -> Z.
+Axiom CRC_range : forall data, 0 <= CRC data < NUM_ENTRY.
 
 Definition process (rw data : Z) (bst : bloomfilter_state) : (bloomfilter_state * Z) :=
   if rw =? 2 then
-    (bloomfilter.add 'I_NUM_ENTRY (fun x y => Nat.eqb x y) CRC CRC CRC bst data, 2)
+    (bloomfilter.add Z Z.eqb CRC CRC CRC bst data, 2)
   else
-    (bst, bool_to_Z (bloomfilter.query 'I_NUM_ENTRY CRC CRC CRC bst data)).
+    (bst, bool_to_Z (bloomfilter.query Z CRC CRC CRC bst data)).
 
 Definition post_arg_assertion : arg_assertion :=
   let (bst', rw') := process rw data bst in
   [
     ArgVal (0%Z, ["myHeader"; "rw"]) (ValBaseBit 8%nat rw');
-    ArgVal (0%Z, ["myHeader"; "data"]) (ValBaseBit 16%nat data)
+    ArgVal (0%Z, ["myHeader"; "data"]) (ValBaseBit 16%nat data);
+    ArgVal (2%Z, ["egress_spec"]) (ValBaseBit 9%nat 1);
+    ArgType (0%Z, []) (TypTypeName (BareName !"headers"));
+    ArgType (1%Z, []) (TypTypeName (BareName !"custom_metadata_t"));
+    ArgType (2%Z, []) (TypTypeName (BareName !"standard_metadata_t"))
   ].
 
 Definition post_ext_assertion : ext_assertion :=
   let (bst', rw') := process rw data bst in
   [
-    (LGlobal !["bloom0"], ObjRegister (mk_register 1%nat (Z.of_nat NUM_ENTRY) (bloom0 bst')));
-    (LGlobal !["bloom1"], ObjRegister (mk_register 1%nat (Z.of_nat NUM_ENTRY) (bloom1 bst')));
-    (LGlobal !["bloom2"], ObjRegister (mk_register 1%nat (Z.of_nat NUM_ENTRY) (bloom2 bst')))
+    (LGlobal !["bloom0"], ObjRegister (mk_register 1%nat NUM_ENTRY (bloom0 bst')));
+    (LGlobal !["bloom1"], ObjRegister (mk_register 1%nat NUM_ENTRY (bloom1 bst')));
+    (LGlobal !["bloom2"], ObjRegister (mk_register 1%nat NUM_ENTRY (bloom2 bst')))
   ].
 
 Definition post (args : list Val) (ret : Val) (st : state) :=
   arg_to_shallow_assertion post_arg_assertion args /\
-    ext_to_shallow_assertion this post_ext_assertion (snd st).
+    to_shallow_assertion_continue this ([], post_ext_assertion) st.
 
 Lemma body_bloomfilter : hoare_func ge inst_m this pre MyIngress_fundef nil post.
 Proof.
   apply deep_hoare_func_sound.
   eapply deep_hoare_func_internal.
+  { (* copy_in *)
+    eapply hoare_copy_in_sound with (pre := (_, (_, _))).
+    repeat constructor.
+  }
+  { (* init block *)
+    simpl eval_copy_in.
+    constructor. apply implies_sound, implies_refl.
+  }
+  {
+    eapply deep_hoare_block_cons.
+    eapply deep_hoare_stmt_if_true.
+    { (* hdr.myHeader.isValid() == true *)
+      admit.
+    }
+    eapply deep_hoare_stmt_block.
+    eapply deep_hoare_block_cons with (mid := Hoare.mk_post_assertion _ _).
+    eapply deep_hoare_stmt_method_call.
+    eapply deep_hoare_call_sound.
+    eapply deep_hoare_call_func.
+    { (* deep_hoare_outargs *)
+      eapply hoare_outargs_sound.
+      repeat constructor.
+    }
+    { (* deep_hoare_inargs *)
+      eapply hoare_inargs_sound.
+      repeat constructor.
+    }
+    { (* lookup_func *)
+      constructor.
+    }
+    { (* deep_hoare_func *)
+      eapply deep_hoare_func_internal (* with
+        (post := to_shallow_arg_ret_assertion this ([], [], ([
+          AVal (LInstance !["hdr"], ["myHeader"; "rw"]) (ValBaseBit 8 rw);
+          AVal (LInstance !["hdr"], ["myHeader"; "data"]) (ValBaseBit 16 data);
+          AVal (LInstance !["standard_metadata"], ["egress_spec"]) (ValBaseBit 9 (P4Arith.BitArith.mod_bound 9 1));
+          AType (LInstance !["hdr"], []) (TypTypeName (BareName !"headers"));
+          AType (LInstance !["meta"], []) (TypTypeName (BareName !"custom_metadata_t"));
+          AType (LInstance !["standard_metadata"], []) (TypTypeName (BareName !"standard_metadata_t"))]
+          ,
+          pre_ext_assertion))) *).
+      { (* copy_in *)
+        eapply hoare_copy_in_sound.
+        repeat constructor.
+      }
+      { (* init block *)
+        simpl eval_copy_in.
+        constructor. apply implies_sound, implies_refl.
+      }
+      { (* body block *)
+        eapply deep_hoare_block_cons with (mid := Hoare.mk_post_assertion _ _).
+        eapply hoare_stmt_sound with (post := mk_post_assertion _ _).
+        { (* wellformed *)
+          constructor.
+        }
+        eapply hoare_stmt_assignment.
+        { (* hoare_lexpr *)
+          constructor.
+        }
+        { (* hoare_expr *)
+          constructor.
+        }
+        { (* hoare_write *)
+          constructor.
+          { (* is_writable_lval *)
+            admit. (* from type *)
+          }
+          constructor.
+        }
+        eapply deep_hoare_block_nil.
+        eapply Hoare.implies_trans.
+        {
+          eapply hoare_copy_out_sound.
+          repeat constructor.
+        }
+        apply Hoare.implies_refl.
+      }
+    }
+    { (* deep_hoare_write_copy_out *)
+      simpl fst. simpl snd.
+      eapply hoare_write_copy_out_sound.
+      repeat constructor.
+    }
+    { (* ret_assertion_to_assertion *)
+      simpl fold_left.
+      eapply ret_assertion_to_assertion_sound.
+      constructor.
+    }
+    {
 (* Qed. *)
 Abort.
 
